

1)

$$\begin{aligned} a) \quad \| \langle -3, 4 \rangle \| &= \sqrt{(-3)^2 + (4)^2} \\ &= \sqrt{9 + 16} \\ &= \sqrt{25} = 5 \end{aligned}$$

b)

$$\begin{aligned} \| \langle -1, 0, 1 \rangle \| &= \sqrt{(-1)^2 + 0^2 + 1^2} \\ &= \sqrt{2} \end{aligned}$$

$$\begin{aligned} c) \quad \| \langle 3, 0, -4 \rangle \| &= \sqrt{3^2 + 0^2 + (-4)^2} \\ &= \sqrt{9 + 16} \\ &= 5 \end{aligned}$$

$$d) \quad \| \langle 5, -2, -2 \rangle \|^2$$

$$= \sqrt{5^2 + (-2)^2 + (-2)^2}$$

$$= \sqrt{25 + 4 + 4}$$

$$= \sqrt{33}$$

2)

a) $\langle -3, 4 \rangle$

$$\vec{u} = \frac{\langle -3, 4 \rangle}{\|\langle -3, 4 \rangle\|} = \boxed{\frac{-3\vec{i} + 4\vec{j}}{5}}$$

b) $\langle -1, 0, 1 \rangle$

$$\vec{u} = \frac{\langle -1, 0, 1 \rangle}{\|\langle -1, 0, 1 \rangle\|} = \frac{-\vec{i} + \vec{k}}{\sqrt{2}} = \boxed{\frac{-\sqrt{2}\vec{i} + \sqrt{2}\vec{k}}{2}}$$

c) $\langle 1, 1, -1 \rangle$

$$\vec{u} = \frac{\langle 1, 1, -1 \rangle}{\|\langle 1, 1, -1 \rangle\|} = \frac{\vec{i} + \vec{j} - \vec{k}}{\sqrt{1^2 + 1^2 + 1^2}} = \boxed{\frac{\vec{i} + \vec{j} - \vec{k}}{3}}$$

d) $\langle 0, -3, 3 \rangle$

$$\begin{aligned} \vec{u} &= \frac{\langle 0, -3, 3 \rangle}{\|\langle 0, -3, 3 \rangle\|} = \frac{\langle 0, -3, 3 \rangle}{\sqrt{0^2 + (-3)^2 + 3^2}} \\ &= \boxed{\frac{-3\vec{j} + 3\vec{k}}{\sqrt{18}}} \end{aligned}$$

$$u \cdot v = \|u\| \|v\| \cos \theta$$

3) a) Angle between $\langle 4, 3 \rangle$ & $\langle 2, -1 \rangle$

$$\Rightarrow (4i + 3j) \cdot (2i - j) = \|\langle 4, 3 \rangle\| \|\langle 2, -1 \rangle\| \cos \theta$$

$$\Rightarrow 8 - 3 = (\sqrt{4^2 + 3^2}) (\sqrt{2^2 + (-1)^2}) \cos \theta$$

$$\Rightarrow 5 = \sqrt{25} \sqrt{5} \cos \theta$$

$$\Rightarrow \cos \theta = 1$$

$$\Rightarrow \theta = \cos^{-1}(1)$$

$$\Rightarrow \theta = 2\pi k, \quad k \in \mathbb{Z}$$

b) Angle between $\langle 1, -4, 1 \rangle$ & $\langle 2, 0, -2 \rangle$

$$\langle 1, -4, 1 \rangle \cdot \langle 2, 0, -2 \rangle = \|\langle 1, -4, 1 \rangle\| \|\langle 2, 0, -2 \rangle\| \cos \theta$$

$$2 + 0 - 2 = \sqrt{1 + 16 + 1} \sqrt{4 + 0 + 4} \cos \theta$$

$$0 = \sqrt{18} \sqrt{8} \cos \theta$$

$$\Rightarrow \cos \theta = 0$$

$$\Rightarrow \theta = 2\pi k, \quad k \in \mathbb{Z}$$

$$\Rightarrow \theta = \begin{cases} \frac{\pi}{2} + 2\pi k \\ -\frac{\pi}{2} + 2\pi k \end{cases}, \quad k \in \mathbb{Z}$$

$$\pi - \frac{\pi}{3} \quad \frac{2\pi}{3}$$

c) Angle between

$$\langle 1, 0, \sqrt{3} \rangle \text{ \& } \langle -1, 0, 0 \rangle$$

$$\langle 1, 0, \sqrt{3} \rangle \cdot \langle -1, 0, 0 \rangle = \|\langle 1, 0, \sqrt{3} \rangle\| \|\langle -1, 0, 0 \rangle\| \cos \theta$$

$$-1 + 0 + 0 = (\sqrt{1+0+3}) (\sqrt{1+0+0}) \cos \theta$$

$$-1 = 2 \cos \theta$$

$$\Rightarrow \cos \theta = -\frac{1}{2}$$

$$\theta = \begin{cases} \frac{2\pi}{3} + 2\pi k \\ -\frac{2\pi}{3} + 2\pi k \end{cases} \quad k \in \mathbb{Z}$$

$$4) a) \langle 2, 3, 0 \rangle \times \langle 1, 0, 5 \rangle = \begin{vmatrix} \hat{i} & \hat{j} & \hat{k} \\ 2 & 3 & 0 \\ 1 & 0 & 5 \end{vmatrix}$$

$$\Rightarrow \hat{i}(15) - \hat{j}(10) + \hat{k}(-3)$$

$$\boxed{15\hat{i} - 10\hat{j} - 3\hat{k}}$$

$$b) \langle 1, 0, 5 \rangle \times \langle 2, 3, 0 \rangle = \begin{vmatrix} \hat{i} & \hat{j} & \hat{k} \\ 1 & 0 & 5 \\ 2 & 3 & 0 \end{vmatrix}$$

$$= \hat{i}(-15) - \hat{j}(-10) + \hat{k}(3)$$

$$= \boxed{-15\hat{i} + 10\hat{j} + 3\hat{k}}$$

$$c) \langle 1, 0, 1 \rangle \times \langle 0, 1, 0 \rangle$$

$$= \begin{vmatrix} \hat{i} & \hat{j} & \hat{k} \\ 1 & 0 & 1 \\ 0 & 1 & 0 \end{vmatrix}$$

$$\hat{i}(-1) - \hat{j}(0) + \hat{k}(1)$$

$$= \boxed{-\hat{i} + \hat{k}}$$

$$d) \langle 2, -1, 1 \rangle \times \langle 4, -2, 2 \rangle = \begin{vmatrix} \hat{i} & \hat{j} & \hat{k} \\ 2 & -1 & 1 \\ 4 & -2 & 2 \end{vmatrix}$$

$$= \hat{i}(-2+2) - \hat{j}(4-4) + \hat{k}(-4+4)$$

$$= \boxed{0}$$

5) Area of triangle with vertices

$$A(1, 0, 0), B(-2, 1, 3), C(4, 2, 5)$$

$$\text{Area} = \frac{1}{2} \|AB \times AC\|$$

$$AB = B - A = (-2, 1, 3) - (1, 0, 0) \\ = (-3, 1, 3)$$

$$AC = C - A = (4, 2, 5) - (1, 0, 0) \\ = (3, 2, 5)$$

$$AB \times AC = \begin{vmatrix} i & j & k \\ -3 & 1 & 3 \\ 3 & 2 & 5 \end{vmatrix} = i(5-6) - j(-15-9) + k(-6-3) \\ = -i + 24j - 9k.$$

$$\|AB \times AC\| = \sqrt{1^2 + 24^2 + 81^2} = \sqrt{658}$$

$$\Rightarrow \boxed{\text{Area} = \frac{1}{2} \sqrt{658}}$$

$$1+3(3)+1$$